proved it in an hour

src/Linker.v
@@ -1,16 +1,241 @@
 Require Import compcert.lib.Coqlib.
 Require Import compcert.common.AST.
+Require Import compcert.common.Globalenvs.
 
 Require Import Oeuf.
 Require Import CompilationUnit.
 
+Require Import StructTact.StructTactics.
+Require Import StructTact.Util.
+Require Import EricTact.
+
+
+(* linker needs to make each id point to only one thing *)
+(* for each id that both have, one needs to be internal, and one needs to be external *)
+(* and we take the internal version *)
+
+(* Only allow calls from shim into Oeuf, not other way around *)
+(* thus internal always on left *)
+Definition link_fundef (a b : Cminor.fundef) : option Cminor.fundef :=
+  match a, b with
+  | Internal _, External ef => (* Oeuf defined function linked against shim *)
+    match ef with
+    | EF_external id sg => Some a
+    | _ => None
+    end
+  | External ef, External ef' => (* common external function, e.g. malloc *)
+    if external_function_eq ef ef' then Some (External ef) else None
+  | _ , _ => None
+  end.
+
+Fixpoint lookup {A} (id : ident) (l : list (ident * A)) : option A :=
+  match l with
+  | nil => None
+  | (id',x) :: r =>
+    if peq id id' then Some x else lookup id r
+  end.
+
+Fixpoint remove_id {A} (id : ident) (l : list (ident * A)) : list (ident * A) :=
+  match l with
+  | nil => nil
+  | (id',x) :: r =>
+    if peq id id' then remove_id id r else (id',x) :: remove_id id r
+  end.
+
+Fixpoint link_fundefs (l l' : list (ident * globdef Cminor.fundef unit)) : option (list (ident * globdef Cminor.fundef unit)) :=
+  match l with
+  | nil => Some l'
+  | (id,Gvar _) :: _ => None
+  | (id,Gfun fd) :: r =>
+    match lookup id l' with
+    | Some (Gfun fd') =>
+      match link_fundef fd fd' with
+      | Some fd0 =>
+        match link_fundefs r (remove_id id l') with
+        | Some l0 => Some ((id,(Gfun fd0)) :: l0)
+        | None => None
+        end
+      | None => None
+      end
+    | _ => None
+    end
+  end.
+    
+           
 (* We need a way to construct a shim, given Oeuf code *)
 Definition shim_link (oeuf_code : Cminor.program) (shim_code : Cminor.program) : option Cminor.program :=
-  if list_norepet_dec peq (prog_defs_names oeuf_code ++ prog_defs_names shim_code) then
-    Some (AST.mkprogram (prog_defs oeuf_code ++ prog_defs shim_code)
-                        (prog_public shim_code)
-                        (prog_main shim_code))
+  if (list_norepet_dec peq (prog_defs_names oeuf_code)) then
+    if (list_norepet_dec peq (prog_defs_names shim_code)) then
+  match (link_fundefs (prog_defs oeuf_code) (prog_defs shim_code)) with
+  | Some fds => Some (AST.mkprogram fds
+                                    (prog_public shim_code)
+                                    (prog_main shim_code))
+  | None => None
+  end
+    else None
   else None.
 
+Lemma remove_id_preserve_not_in :
+  forall {A} (l : list (ident * A)) i,
+    ~ In i (map fst l) ->
+    forall id,
+      ~ In i (map fst (remove_id id l)).
+Proof.
+  induction l; intros.
+  simpl in *. eauto.
+  simpl in *. eapply Decidable.not_or in H.
+  break_and.
+  destruct a. break_match; try subst.
+  eapply IHl; eauto.
+  simpl.
+  intro. eapply H0. break_or. subst. simpl in H. congruence.
+  eapply IHl in H0. eapply H0 in H1. inversion H1.
+Qed.
 
-(* In the future, maybe we define the rest of the Oeuf compiler here *)
+Lemma link_fundefs_not_in :
+  forall a b l,
+    link_fundefs a b = Some l ->
+    forall i,
+      ~ In i (map fst a) ->
+      ~ In i (map fst b) ->
+      ~ In i (map fst l).
+Proof.
+  induction a; intros.
+  simpl in *. inv H. eauto.
+  simpl in *. repeat (break_match_hyp; try congruence).
+  eapply Decidable.not_or in H0.
+  break_and. simpl in *.
+  invc H.
+  simpl.
+  intro. break_or; try congruence.
+  eapply IHa; eauto.
+  eapply remove_id_preserve_not_in; eauto.
+Qed.
+
+Lemma remove_id_not_in :
+  forall {A} id (l : list (ident * A)),
+    ~ In id (map fst (remove_id id l)).
+Proof.
+  induction l; intros.
+  simpl. eauto.
+  simpl in *. destruct a.
+  break_match. subst. eauto.
+  simpl. intro. eapply IHl.
+  break_or; congruence.
+Qed.
+
+Lemma list_norepet_remove_id :
+  forall {A} (l : list (ident * A)),
+    list_norepet (map fst l) ->
+    forall id,
+      list_norepet (map fst (remove_id id l)).
+Proof.
+  induction l; intros;
+    simpl in *; eauto.
+  destruct a. break_match. subst.
+  simpl in *. inv H.
+  eauto.
+  simpl in *.
+  inv H.
+  eapply IHl in H3; eauto.
+  econstructor; eauto.
+  eapply remove_id_preserve_not_in; eauto.
+Qed.
+
+Lemma link_fundefs_norepet :
+  forall a b c,
+    list_norepet (map fst a) ->
+    list_norepet (map fst b) ->
+    link_fundefs a b = Some c ->
+    list_norepet (map fst c).
+Proof.
+  induction a; intros.
+  simpl in H1. inv H1. assumption.
+  simpl in *. repeat (break_match_hyp; try congruence).
+  subst. inv H1. simpl in *.
+  inv H. econstructor; eauto.
+  eapply link_fundefs_not_in; eauto.
+  eapply remove_id_not_in.
+  eapply IHa. eauto.
+  Focus 2. eassumption.
+  eapply list_norepet_remove_id; eauto.
+Qed.
+
+Lemma list_norepet_link :
+  forall a b c,
+    shim_link a b = Some c ->
+    list_norepet (prog_defs_names c).
+Proof.
+  intros. unfold shim_link in *.
+  repeat break_match_hyp; try congruence.
+  inv H. unfold prog_defs_names.
+  eapply link_fundefs_norepet in Heqo; eauto.
+Qed.
+
+Lemma link_fundef_left :
+  forall a b c,
+    link_fundef a b = Some c ->
+    a = c.
+Proof.
+  intros.
+  unfold link_fundef in *;
+    repeat (break_match_hyp; try congruence).
+Qed.
+
+Lemma prog_def_link_fundefs :
+  forall a b c,
+    link_fundefs a b = Some c ->
+    forall id fd,
+      In (id,Gfun fd) a ->
+      In (id,Gfun fd) c.
+Proof.
+  induction a; intros; simpl in *.
+  inv H0.
+  repeat (break_match_hyp; try congruence). subst.
+  invc H.
+  break_or. invc H.
+  simpl. left.
+  app link_fundef_left link_fundef. subst.
+  reflexivity.
+  simpl. right.
+  eapply IHa; eauto.
+Qed.
+      
+
+Lemma prog_def_transf :
+  forall a b c,
+    shim_link a b = Some c ->
+    forall id fd,
+      In (id,Gfun fd) (prog_defs a) ->
+      In (id,Gfun fd) (prog_defs c).
+Proof.
+  intros.
+  unfold shim_link in *.
+  repeat (break_match_hyp; try congruence).
+  inv H. simpl.
+  eapply prog_def_link_fundefs; eauto.
+Qed.
+
+Section LINKED.
+
+  Variable oeuf_code shim_code link_code : Cminor.program.
+  Hypothesis TRANSF : shim_link oeuf_code shim_code = Some link_code.
+
+  Definition oeuf_ge := Genv.globalenv oeuf_code.
+  Definition shim_ge := Genv.globalenv shim_code.
+  Definition link_ge := Genv.globalenv link_code.
+  
+  Lemma oeuf_ident_transf :
+    forall id fd,
+      (exists b, Genv.find_symbol oeuf_ge id = Some b /\ Genv.find_funct_ptr oeuf_ge b = Some fd) ->
+      (exists b, Genv.find_symbol link_ge id = Some b /\ Genv.find_funct_ptr link_ge b = Some fd).
+  Proof.
+    intros.
+    break_exists. break_and.
+    app Genv.find_funct_ptr_symbol_inversion Genv.find_symbol.
+    eapply Genv.find_funct_ptr_exists; eauto.
+    eapply list_norepet_link; eauto.
+    eapply prog_def_transf; eauto.
+  Qed.
+
+End LINKED.
